examples/lpr_checker/array/compilation/README.md
@@ -2,3 +2,6 @@ An LRAT checker built on CakeML with arrays
 
 [lrat_arrayCompileScript.sml](lrat_arrayCompileScript.sml):
 Compiles the lrat example by evaluation inside the logic of HOL
+
+[proofs](proofs):
+Prove end-to-end correctness theorem for LRAT checker with arrays
